used FTLR in the adequacy proof

lawyer/nonblocking/logrel/fundamental.v
@@ -2,7 +2,7 @@
 (* From iris.program_logic Require Export weakestpre. *)
 
 From iris.proofmode Require Import proofmode coq_tactics.
-From lawyer.nonblocking.logrel Require Export persistent_pred logrel substitutions.
+From lawyer.nonblocking.logrel Require Export persistent_pred logrel substitutions valid_client.
 From lawyer.nonblocking Require Export pwp. 
 From iris.base_logic Require Import invariants.
 From iris.prelude Require Import options.
@@ -115,44 +115,6 @@ Section typed_interp.
   Ltac inv_unop_eval H :=
     apply un_op_eval_inv in H as
         [(-> & ? & -> & ->) | [(-> & ? & -> & ->)| (-> & ? & -> & ->)]]. 
-
-  Definition valid_base_lit (v: base_lit) : Prop :=
-    match v with
-    | LitInt _ | LitBool _ | LitUnit => True
-    | LitLoc _ | LitProphecy _ | LitPoison => False
-  end.
-
-  Definition valid_bin_op (op: bin_op): Prop :=
-    match op with 
-    | OffsetOp => False
-    | _ => True
-    end. 
-
-  (* a valid client proram is any program without:
-     - hard-coded locations
-     - address offset operations
-     TODO: currently we also exclude prophecies, seems reasonable? *)
-  Fixpoint valid_client (e : expr) : Prop :=
-    match e with
-    | Val v => valid_val v
-    | Var _ | ChooseNat => True
-    | Rec _ _  e | UnOp _ e | Fst e | Snd e |
-      InjL e | InjR e | Fork e | Load e
-      => valid_client e
-    | App e1 e2 | Pair e1 e2 | 
-      AllocN e1 e2 | Store e1 e2 | FAA e1 e2
-      => valid_client e1 /\ valid_client e2
-    | BinOp op e1 e2 => valid_bin_op op /\ valid_client e1 /\ valid_client e2
-    | If e0 e1 e2 | Case e0 e1 e2 | CmpXchg e0 e1 e2
-      => valid_client e0 /\ valid_client e1 /\ valid_client e2
-    end
-  with valid_val (v: val) : Prop :=
-    match v with
-    | LitV b => valid_base_lit b
-    | RecV _ _ e => valid_client e
-    | PairV v1 v2 => valid_val v1 /\ valid_val v2
-    | InjLV v | InjRV v => valid_val v
-    end.
 
   Lemma logrel_var x : ⊢ logrel (Var x).
   Proof.
