lawyer/nonblocking/logrel/valid_client.v
@@ -1,0 +1,39 @@
+From heap_lang Require Import heap_lang_defs sswp_logic tactics. 
+
+Definition valid_base_lit (v: base_lit) : Prop :=
+  match v with
+  | LitInt _ | LitBool _ | LitUnit => True
+  | LitLoc _ | LitProphecy _ | LitPoison => False
+  end.
+
+Definition valid_bin_op (op: bin_op): Prop :=
+  match op with 
+  | OffsetOp => False
+  | _ => True
+  end. 
+
+(* a valid client proram is any program without:
+     - hard-coded locations
+     - address offset operations
+     TODO: currently we also exclude prophecies, seems reasonable? *)
+Fixpoint valid_client (e : expr) : Prop :=
+  match e with
+  | Val v => valid_val v
+  | Var _ | ChooseNat => True
+  | Rec _ _  e | UnOp _ e | Fst e | Snd e |
+    InjL e | InjR e | Fork e | Load e
+    => valid_client e
+  | App e1 e2 | Pair e1 e2 | 
+    AllocN e1 e2 | Store e1 e2 | FAA e1 e2
+    => valid_client e1 /\ valid_client e2
+  | BinOp op e1 e2 => valid_bin_op op /\ valid_client e1 /\ valid_client e2
+  | If e0 e1 e2 | Case e0 e1 e2 | CmpXchg e0 e1 e2
+    => valid_client e0 /\ valid_client e1 /\ valid_client e2
+  end
+with valid_val (v: val) : Prop :=
+  match v with
+  | LitV b => valid_base_lit b
+  | RecV _ _ e => valid_client e
+  | PairV v1 v2 => valid_val v1 /\ valid_val v2
+  | InjLV v | InjRV v => valid_val v
+end.
